Updated so that invol proofs go through

src/JSON_Core.v
@@ -6,10 +6,12 @@ Require Coq.Program.Wf.
 Require Import Lia.
 
 Import ListNotations.
+Import ResultNotation.
 
 Open Scope string_scope.
 
 Ltac jsonifiable_hammer := 
+  intros;
   repeat break_match; simpl in *; try congruence;
   repeat find_injection; simpl in *; try congruence;
   repeat rewrite canonical_stringification in *; try congruence; try find_injection; try auto;
@@ -67,25 +69,27 @@ Proof.
 Defined.
 
 Definition ASP_PARAMS_to_JSON `{Jsonifiable ASP_ARGS} (t : ASP_PARAMS) : JSON := 
-    match t with
-    | asp_paramsC asp_id args plc targ_id => 
-        JSON_Object [
-          ("ASP_ID", JSON_String (to_string asp_id));
-          ("ASP_ARGS", (to_JSON args));
-          ("ASP_PLC", JSON_String (to_string plc));
-          ("ASP_TARG_ID", JSON_String (to_string targ_id))
-        ]
-    end.
+  match t with
+  | asp_paramsC asp_id args plc targ_id => 
+      JSON_Object [
+        ("ASP_ID", JSON_String (to_string asp_id));
+        ("ASP_ARGS", (to_JSON args));
+        ("ASP_PLC", JSON_String (to_string plc));
+        ("ASP_TARG_ID", JSON_String (to_string targ_id))
+      ]
+  end.
 
 Definition ASP_PARAMS_from_JSON `{Jsonifiable ASP_ARGS} (js : JSON) : ResultT ASP_PARAMS string :=
-  match (JSON_get_Object "ASP_ID" js), (JSON_get_Object "ASP_ARGS" js), (JSON_get_Object "ASP_PLC" js), (JSON_get_Object "ASP_TARG_ID" js) with
-  | resultC (JSON_String asp_id), resultC args, resultC (JSON_String plc), resultC (JSON_String targ_id) => 
-      match (from_string asp_id), (from_JSON args), (from_string plc), (from_string targ_id) with
-      | resultC asp_id, resultC args, resultC plc, resultC targ_id => resultC (asp_paramsC asp_id args plc targ_id)
-      | _, _, _, _ => errC "Parsing ASP_PARAMS not successful"
-      end
-  | _, _, _, _ => errC "Invalid ASP_PARAMS JSON"
-  end.
+  asp_id  <- JSON_get_string "ASP_ID" js ;;
+  args    <- JSON_get_Object "ASP_ARGS" js ;;
+  plc     <- JSON_get_string "ASP_PLC" js ;;
+  targ    <- JSON_get_string "ASP_TARG_ID" js ;;
+
+  asp_id' <- from_string asp_id ;;
+  args'   <- from_JSON args ;;
+  plc'    <- from_string plc ;;
+  targ'   <- from_string targ ;;
+  resultC (asp_paramsC asp_id' args' plc' targ').
 
 Global Instance Jsonifiable_ASP_Params `{Jsonifiable ASP_ARGS} : Jsonifiable ASP_PARAMS. 
 eapply Build_Jsonifiable with 
@@ -96,7 +100,6 @@ unfold ASP_PARAMS_from_JSON;
 intuition; simpl in *;
 jsonifiable_hammer.
 Defined.
-
 
 Definition type_string_constant : string := "CONSTRUCTOR".
 Definition body_string_constant : string := "BODY".
@@ -150,20 +153,16 @@ eapply Build_Jsonifiable with
                     end
                   | _ => errC "Invalid nat JSON (not a JSON String)"
                   end)).
-intros.
-break_match;
-rewrite canonical_stringification in *; 
-try congruence.
+jsonifiable_hammer.
 Defined.
 
 Definition constructor_body_from_JSON_gen (type_name:string) (js:JSON) 
-    : list JSON.
-  refine ((match (JSON_get_Object (type_name ++ "_" ++ body_string_constant) js) as m' return m' = (JSON_get_Object (type_name ++ "_" ++ body_string_constant) js) -> list JSON with
-  | resultC (JSON_Array ls) => fun Heq => ls  (* 2+ constructor args case *)
-  | resultC jv => fun Heq => [jv]             (* 1 arg case *)
-  | errC _ => fun Heq => nil                   (* 0 args case *)
-  end) eq_refl).
-Defined.
+    : list JSON :=
+  match (JSON_get_Object (type_name ++ "_" ++ body_string_constant) js) with
+  | resultC (JSON_Array ls) => ls  (* 2+ constructor args case *)
+  | resultC jv => [jv]             (* 1 arg case *)
+  | errC _ => nil                   (* 0 args case *)
+  end.
 
 Definition from_JSON_gen {A:Type} (type_name:string) 
   (cmap: (MapC string (JSON -> (ResultT A string)))) 
@@ -298,7 +297,7 @@ Proof.
       repeat rewrite String.eqb_neq in *; subst; jsonifiable_hammer;
       try rewrite String.eqb_eq in *; unfold type_string_constant,
       body_string_constant in *;
-      try rewrite string_app_helper in *; try congruence.
+      try rewrite string_app_helper in *; try congruence;
       exfalso; eauto.
     * (* ls = [j] *)
       jsonifiable_hammer;
@@ -341,287 +340,56 @@ Fixpoint Evidence_to_JSON `{Jsonifiable FWD, Jsonifiable nat, Jsonifiable ASP_PA
         [(Evidence_to_JSON e1); (Evidence_to_JSON e2)]
   end.
 
-Definition nn_args_from_json (ls: list JSON) : ResultT Evidence string := 
-  match ls with 
-  | [(JSON_String n_str)] => 
-      match (from_string n_str) with
-      | resultC n => resultC (nn n)
-      | errC e => errC e
-      end
-  | [_] => errC ("JSON Parsing " ++ nn_name_constant ++ " ARGS:  wrong JSON arg type (expected JSON_String)")
-  | _ =>   errC ("JSON Parsing " ++ nn_name_constant ++ " ARGS:  wrong number of JSON args (expected 1)")
-  end.
-
-Definition ss_args_from_json {top_js} (recf: forall y : JSON, JSON_depth y < JSON_depth top_js -> ResultT Evidence string) (ls : {ls : list JSON
-  | forall y : JSON, In y ls -> JSON_depth y < JSON_depth top_js}) {HLT : exists s', JSON_get_Object s' top_js = resultC (JSON_Array (proj1_sig ls))}: ResultT Evidence string.
-  refine ((match (proj1_sig ls) as ls' return (proj1_sig ls) = ls' -> ResultT Evidence string with
-  | [ ev1; 
-      ev2 ] => 
-      fun Heq =>
-      match (recf ev1 _), (recf ev2 _) with
-      | resultC evres1, resultC evres2 => resultC (ss evres1 evres2)
-      | _, _ => errC "other"
-      end
-  | [_] => fun _ => errC ("JSON Parsing " ++ nn_name_constant ++ " ARGS:  wrong JSON arg type (expected JSON_String)")
-  | _ =>   fun _ => errC ("JSON Parsing " ++ nn_name_constant ++ " ARGS:  wrong number of JSON args (expected 1)")
-  end) eq_refl); subst; simpl in *; eauto;
-  break_exists; find_apply_lem_hyp json_get_object_result_always_smaller; 
-  eapply PeanoNat.Nat.lt_trans; try eassumption;
-  eapply json_all_array_elements_smaller; 
-  rewrite Heq; simpl; eauto.
-Defined.
-
-Definition uu_args_from_json {top_js} (recf: forall y : JSON, JSON_depth y < JSON_depth top_js -> ResultT Evidence string) (ls : {ls : list JSON
-  | forall y : JSON, In y ls -> JSON_depth y < JSON_depth top_js}) {HLT : exists s', JSON_get_Object s' top_js = resultC (JSON_Array (proj1_sig ls))}: ResultT Evidence string.
-  refine ((
-    match (proj1_sig ls) as ls' return (proj1_sig ls) = ls' -> ResultT Evidence string with 
-  | [(JSON_String plc);
-      fwd;
-      asp_par; 
-      ev' ] => 
-      fun Heq =>
-      match (from_string plc), (from_JSON fwd), (from_JSON asp_par), (recf ev' _) with
-      | resultC plcres, resultC fwdres, resultC parres, resultC evres => resultC (uu plcres fwdres parres evres)
-      | _, _, _, _ => errC "other"
-      end
-  | [_] => fun _ => errC ("JSON Parsing " ++ nn_name_constant ++ " ARGS:  wrong JSON arg type (expected JSON_String)")
-  | _ =>  fun _ => errC ("JSON Parsing " ++ nn_name_constant ++ " ARGS:  wrong number of JSON args (expected 1)")
-  end) eq_refl); subst; simpl in *; eauto.
-  destruct HLT.
-  eapply json_get_object_result_always_smaller in H as H'.
-  eapply PeanoNat.Nat.lt_trans; [ | eauto].
-  - eapply json_all_array_elements_smaller.
-    rewrite Heq; simpl in *; subst; eauto. 
-Defined.
-
-Lemma json_depth_order_wf : well_founded (fun x y => lt (JSON_depth x) (JSON_depth y)).
-Proof.
-  eapply Wf_nat.well_founded_ltof.
-Defined.
-
-
-
-Definition Evidence_from_JSON `{Jsonifiable FWD, Jsonifiable nat, Jsonifiable ASP_PARAMS} (js : JSON) : ResultT Evidence string.
-generalize js.
-refine (Fix json_depth_order_wf (fun _ => ResultT Evidence string)
-  (
-    fun (js : JSON)
-      (rec : forall y : JSON,
-             lt (JSON_depth y) (JSON_depth js) ->
-             ResultT Evidence string) =>
+Fixpoint Evidence_from_JSON `{Jsonifiable FWD, Jsonifiable nat, Jsonifiable ASP_PARAMS} (js : JSON) : ResultT Evidence string :=
     let type_name := evidence_name_constant in
     match (JSON_get_Object (type_name ++ "_" ++ type_string_constant) js) with
     | resultC (JSON_String cons_name) =>
       if (eqb cons_name mt_name_constant) 
       then resultC mt
       else if (eqb cons_name nn_name_constant) 
-      then 
-          match (JSON_get_Object (type_name ++ "_" ++ body_string_constant) js) as m' return m' = (JSON_get_Object (type_name ++ "_" ++ body_string_constant) js) -> ResultT Evidence string with
-          | resultC n_js => 
-              fun _ =>
-              match (from_JSON n_js) with
-              | resultC n => resultC (nn n)
-              | errC e => errC e
-              end
-          | errC e => fun _ => errC e
-          end eq_refl
+      then match js with
+          | JSON_Object [
+              _;
+              (_, n_js)
+            ] =>
+              n_js <- from_JSON n_js ;;
+              resultC (nn n_js)
+          | _ => errC ("JSON Parsing " ++ nn_name_constant ++ " ARGS:  wrong number of JSON args (expected 1)")
+          end
       else if (eqb cons_name uu_name_constant) 
-      then
-          match (JSON_get_Object (type_name ++ "_" ++ body_string_constant) js) as m' return (JSON_get_Object (type_name ++ "_" ++ body_string_constant) js) = m' -> ResultT Evidence string with
-          | resultC (JSON_Array [
-                JSON_String plc; fwd; asp_par; ev'
-              ]) =>
-                fun _ =>
-                match (from_string plc), (from_JSON fwd), (from_JSON asp_par), (rec ev' _) with
-                | resultC plc, resultC fwd, resultC ps, resultC e =>
-                  resultC (uu plc fwd ps e)
-                | _, _, _, _ => errC "other"
-                end
-          | resultC _ =>  fun _ => errC ("JSON Parsing " ++ uu_name_constant ++ " ARGS:  wrong number of JSON args (expected 4)")
-          | errC e => fun _ => errC e
-          end eq_refl
+      then match js with
+          | JSON_Object [
+              _;
+              (_, JSON_Array [ JSON_String plc; fwd; asp_par; ev' ])
+            ] =>
+              plc <- from_string plc ;;
+              fwd <- from_JSON fwd ;;
+              asp_par <- from_JSON asp_par ;;
+              ev' <- Evidence_from_JSON ev' ;;
+              resultC (uu plc fwd asp_par ev')
+          | _ => errC ("JSON Parsing " ++ uu_name_constant ++ " ARGS:  wrong number of JSON args (expected 4)")
+          end 
       else if (eqb cons_name ss_name_constant) 
-      then  
-          match (JSON_get_Object (type_name ++ "_" ++ body_string_constant) js) as m' return (JSON_get_Object (type_name ++ "_" ++ body_string_constant) js) = m' -> ResultT Evidence string with
-          | resultC (JSON_Array [ ev1; ev2 ]) =>
-              fun _ =>
-                match (rec ev1 _), (rec ev2 _) with
-                | resultC e1, resultC e2 => resultC (ss e1 e2)
-                | _, _ => errC "other"
-                end
-          | resultC _ =>  fun _ => errC ("JSON Parsing " ++ ss_name_constant ++ " ARGS:  wrong number of JSON args (expected 2)")
-          | errC e => fun _ => errC e
-          end eq_refl
-      else errC "Invalid Evidence JSON constructor name"
-    | resultC _ => errC ("Invalid " ++ type_name ++ " JSON:  no constructor name string")
-    | errC e => errC e
-    end)).
-- eapply json_get_object_result_always_smaller in e as E;
-  eapply PeanoNat.Nat.lt_trans; [ | eauto];
-  eapply json_all_array_elements_smaller; eauto;
-  simpl in *; eauto.
-- eapply json_get_object_result_always_smaller in e as E;
-  eapply PeanoNat.Nat.lt_trans; [ | eauto];
-  eapply json_all_array_elements_smaller; eauto;
-  simpl in *; eauto.
-- eapply json_get_object_result_always_smaller in e as E;
-  eapply PeanoNat.Nat.lt_trans; [ | eauto];
-  eapply json_all_array_elements_smaller; eauto;
-  simpl in *; eauto.
-Defined.
-
-(* Definition Evidence_from_JSON_map {top_js} (recf: forall y : JSON, JSON_depth y < JSON_depth top_js -> ResultT Evidence string) {HLT : forall ls, exists s', JSON_get_Object s' top_js = resultC (JSON_Array ls)} : MapC string (JSON -> (ResultT Evidence string)) :=
-  [(mt_name_constant, 
-    constructor_from_JSON evidence_name_constant (fun _ => resultC mt));
-   (nn_name_constant, 
-    constructor_from_JSON evidence_name_constant nn_args_from_json);
-   (uu_name_constant, 
-    fun top_js => @constructor_from_JSON_rec _ top_js evidence_name_constant (
-      fun ls => uu_args_from_json recf ls (HLT (proj1_sig ls))));
-   (ss_name_constant,
-    fun top_js =>
-    constructor_from_JSON_rec evidence_name_constant (
-      fun ls => ss_args_from_json recf ls (HLT (proj1_sig ls))))].
-
-Definition from_JSON_gen_rec {A:Type} (type_name:string) 
-  (cmap: (MapC string (JSON -> (ResultT A string)))) 
-    : JSON -> ResultT A string := 
-  fun js => 
-    match (JSON_get_Object (type_name ++ "_" ++ type_string_constant) js) as m' return m' = (JSON_get_Object (type_name ++ "_" ++ type_string_constant) js) -> ResultT A string with
-    | resultC (JSON_String cons_name) =>
-      match (map_get cmap cons_name) with 
-      | Some f => fun Heq => f js
-      | None => fun _ => errC ("Invalid " ++ type_name ++ " JSON:  unrecognized constructor name: " ++ cons_name)
-      end
-    | resultC _ => fun _ => errC ("Invalid " ++ type_name ++ " JSON:  no constructor name string")
-    | errC e => fun _ => errC e
-    end eq_refl.
-
-
-Program Fixpoint Evidence_from_JSON' (js : JSON) {measure (JSON_depth js)} : ResultT Evidence string :=
-  from_JSON_gen evidence_name_constant (@Evidence_from_JSON_map js Evidence_from_JSON') js. *)
-
-(*
-Definition Evidence_from_JSON' (js : JSON) (m:MapC string (JSON -> (ResultT Evidence string))) : ResultT Evidence string :=
-  from_JSON_gen_nonrec evidence_name_constant m js.
-
-Program Fixpoint Evidence_from_JSON (js : JSON) {measure (JSON_depth js)} : ResultT Evidence string :=
-  Evidence_from_JSON' js (Evidence_from_JSON_map (fun js' => Evidence_from_JSON js')).
-Next Obligation.
-Admitted.
-*)
-
-Definition uu_ev_ex : Evidence := uu "P0" COMP (asp_paramsC "i" [] "P0" "P0") mt.
-
-Definition ss_ev_ex : Evidence := ss uu_ev_ex uu_ev_ex.
-
-Example uuev_ex : (Evidence_from_JSON (Evidence_to_JSON uu_ev_ex) = (resultC uu_ev_ex)).
-Proof.
-  intros.
-  jsonifiable_hammer.
-Qed.
-
-Example ssev_ex : (Evidence_from_JSON (Evidence_to_JSON ss_ev_ex) = (resultC ss_ev_ex)).
-Proof.
-  intros.
-  jsonifiable_hammer.
-Qed.
-
-Theorem Evidence_from_JSON_eq : forall `{Jsonifiable FWD, Jsonifiable nat, Jsonifiable ASP_PARAMS} (js : JSON),
-  Evidence_from_JSON js = 
-    let type_name := evidence_name_constant in
-    match (JSON_get_Object (type_name ++ "_" ++ type_string_constant) js) with
-    | resultC (JSON_String cons_name) =>
-      if (eqb cons_name mt_name_constant) 
-      then resultC mt
-      else if (eqb cons_name nn_name_constant) 
-      then 
-          match (JSON_get_Object (type_name ++ "_" ++ body_string_constant) js) as m' return m' = (JSON_get_Object (type_name ++ "_" ++ body_string_constant) js) -> ResultT Evidence string with
-          | resultC n_js => 
-              fun _ =>
-              match (from_JSON n_js) with
-              | resultC n => resultC (nn n)
-              | errC e => errC e
-              end
-          | errC e => fun _ => errC e
-          end eq_refl
-      else if (eqb cons_name uu_name_constant) 
-      then
-          match (JSON_get_Object (type_name ++ "_" ++ body_string_constant) js) as m' return (JSON_get_Object (type_name ++ "_" ++ body_string_constant) js) = m' -> ResultT Evidence string with
-          | resultC (JSON_Array [
-                JSON_String plc; fwd; asp_par; ev'
-              ]) =>
-                fun _ =>
-                match (from_string plc), (from_JSON fwd), (from_JSON asp_par), (Evidence_from_JSON ev') with
-                | resultC plc, resultC fwd, resultC ps, resultC e =>
-                  resultC (uu plc fwd ps e)
-                | _, _, _, _ => errC "other"
-                end
-          | resultC _ =>  fun _ => errC ("JSON Parsing " ++ uu_name_constant ++ " ARGS:  wrong number of JSON args (expected 4)")
-          | errC e => fun _ => errC e
-          end eq_refl
-      else if (eqb cons_name ss_name_constant) 
-      then  
-          match (JSON_get_Object (type_name ++ "_" ++ body_string_constant) js) as m' return (JSON_get_Object (type_name ++ "_" ++ body_string_constant) js) = m' -> ResultT Evidence string with
-          | resultC (JSON_Array [ ev1; ev2 ]) =>
-              fun _ =>
-                match (Evidence_from_JSON ev1), (Evidence_from_JSON ev2) with
-                | resultC e1, resultC e2 => resultC (ss e1 e2)
-                | _, _ => errC "other"
-                end
-          | resultC _ =>  fun _ => errC ("JSON Parsing " ++ ss_name_constant ++ " ARGS:  wrong number of JSON args (expected 2)")
-          | errC e => fun _ => errC e
-          end eq_refl
+      then match js with
+          | JSON_Object [
+              _;
+              (_, JSON_Array [ ev1; ev2 ])
+           ] =>
+              ev1 <- Evidence_from_JSON ev1 ;;
+              ev2 <- Evidence_from_JSON ev2 ;;
+              resultC (ss ev1 ev2)
+          | _ => errC ("JSON Parsing " ++ ss_name_constant ++ " ARGS:  wrong number of JSON args (expected 2)")
+          end 
       else errC "Invalid Evidence JSON constructor name"
     | resultC _ => errC ("Invalid " ++ type_name ++ " JSON:  no constructor name string")
     | errC e => errC e
     end.
-Proof.
-  intros; apply (Fix_eq json_depth_order_wf (fun _ => ResultT Evidence string)); intros; intuition;
-  repeat (break_match; eauto; intuition; eauto; try congruence;
-    try rewrite String.eqb_eq in *; subst; 
-    try rewrite String.eqb_neq in *; subst; try congruence
-  ).
-  - generalize (eq_refl ((JSON_get_Object (evidence_name_constant ++ "_" ++ body_string_constant) x))).
-    intros.
-    (* Print case_eq.
-  
-  set (X := JSON_get_Object (evidence_name_constant ++ "_" ++ body_string_constant) x) in *.
-    dependent destruction X.
-    * admit.
-    * subst. 
-      dependent rewrite <- x.
-    destruct x; try (simpl in *; congruence).
-    destruct m; try (simpl in *; congruence);
-    destruct p; try (simpl in *; congruence).
-    destruct s; try (simpl in *; congruence);
-    destruct j; try (simpl in *; congruence).
-    *  
-    destruct (JSON_get_Object (evidence_name_constant ++ "_" ++ body_string_constant) x).
-  
-  unfold JSON_get_Object.
-    destruct x.
-    * unfold map_get.
-    destruct (JSON_get_Object (evidence_name_constant ++ "_" ++ body_string_constant) x).
-  
-    generalize (evidence_name_constant ++ "_" ++ body_string_constant).
-    destruct (JSON_get_Object (evidence_name_constant ++ "_" ++ body_string_constant) x) eqn:?.
-    subst.
-    * 
-    set (M := JSON_get_Object X1 x) in *.
-    generalize_eqs M.
-    destruct M.
-    destruct M.
-    destruct (JSON_get_Object X1 x) eqn:?; try congruence;
-    destruct j; try congruence; try find_injection. *)
-
-Admitted.
 
 Global Instance Jsonifiable_Evidence `{Jsonifiable ASP_ARGS, Jsonifiable FWD, Jsonifiable nat, Jsonifiable ASP_PARAMS} : Jsonifiable Evidence.
 eapply Build_Jsonifiable with (to_JSON := Evidence_to_JSON) (from_JSON := Evidence_from_JSON).
-induction a; rewrite Evidence_from_JSON_eq; simpl in *;
-jsonifiable_hammer; repeat rewrite canonical_jsonification in *;
-jsonifiable_hammer.
+induction a; simpl in *;
+repeat (result_monad_unfold;
+jsonifiable_hammer; repeat rewrite canonical_jsonification in *).
 Defined.
 
 Global Instance Stringifiable_SP : Stringifiable SP := {
@@ -735,16 +503,8 @@ Fixpoint Term_to_JSON `{Jsonifiable ASP, Jsonifiable Split} (t : Term) : JSON :=
       [(to_JSON sp); (Term_to_JSON t1); (Term_to_JSON t2)]
   end.
 
-Import ResultNotation.
 
-Definition Term_from_JSON `{Jsonifiable ASP, Jsonifiable Split} (js : JSON) : ResultT Term string.
-generalize js.
-refine (Fix json_depth_order_wf (fun _ => ResultT Term string)
-  (
-    fun (js : JSON)
-      (rec : forall y : JSON,
-             lt (JSON_depth y) (JSON_depth js) ->
-             ResultT Term string) =>
+Fixpoint Term_from_JSON `{Jsonifiable ASP, Jsonifiable Split} (js : JSON) : ResultT Term string :=
     let type_name := "TERM" in
     let type_str := type_name ++ "_" ++ type_string_constant in
     let body_str := type_name ++ "_" ++ body_string_constant in
@@ -756,137 +516,59 @@ refine (Fix json_depth_order_wf (fun _ => ResultT Term string)
         asp_val <- from_JSON asp_js ;;
         resultC (asp asp_val)
       else if (eqb cons_name "att") 
-      then 
-        match (JSON_get_Object body_str js) as m' return (JSON_get_Object body_str js) = m' -> ResultT Term string with
-        | resultC (JSON_Array [JSON_String plc; term']) =>
-            fun _ =>
-            plc_val <- from_string plc ;;
-            term_val <- (rec term' _) ;;
-            resultC (att plc_val term_val)
-        | resultC _ => fun _ => errC ("JSON Parsing 'att' ARGS: Incorrect number or wrong type of JSON args (expected [plc; term])")
-        | errC e => fun _ => errC e
-        end eq_refl
-      else if (eqb cons_name "lseq") 
-      then
-        match (JSON_get_Object body_str js) as m' return (JSON_get_Object body_str js) = m' -> ResultT Term string with
-        | resultC (JSON_Array [ term1; term2 ]) =>
-            fun _ =>
-            term1_val <- (rec term1 _) ;;
-            term2_val <- (rec term2 _) ;;
-            resultC (lseq term1_val term2_val)
-        | resultC _ => fun _ => errC ("JSON Parsing 'lseq' ARGS: Incorrect number or wrong type of JSON args (expected [term1; term2])")
-        | errC e => fun _ => errC e
-        end eq_refl
-      else if (eqb cons_name "bseq") 
-      then  
-        match (JSON_get_Object body_str js) as m' return (JSON_get_Object body_str js) = m' -> ResultT Term string with
-        | resultC (JSON_Array [ sp; term1; term2 ]) =>
-            fun _ =>
-            sp_val <- from_JSON sp ;;
-            term1_val <- (rec term1 _) ;;
-            term2_val <- (rec term2 _) ;;
-            resultC (bseq sp_val term1_val term2_val)
-        | resultC _ => fun _ => errC ("JSON Parsing 'bseq' ARGS: Incorrect number or wrong type of JSON args (expected [sp; term1; term2])")
-        | errC e => fun _ => errC e
-        end eq_refl
-      else if (eqb cons_name "bpar") 
-      then  
-        match (JSON_get_Object body_str js) as m' return (JSON_get_Object body_str js) = m' -> ResultT Term string with
-        | resultC (JSON_Array [ sp; term1; term2 ]) =>
-            fun _ =>
-            sp_val <- from_JSON sp ;;
-            term1_val <- (rec term1 _) ;;
-            term2_val <- (rec term2 _) ;;
-            resultC (bpar sp_val term1_val term2_val)
-        | resultC _ => fun _ => errC ("JSON Parsing 'bpar' ARGS: Incorrect number or wrong type of JSON args (expected [sp; term1; term2])")
-        | errC e => fun _ => errC e
-        end eq_refl
-      else errC "Invalid Term JSON constructor name"
-    | resultC _ => errC "Invalid Term type"
-    | errC e => errC e
-    end)); eapply json_get_object_result_always_smaller in e as E;
-  eapply PeanoNat.Nat.lt_trans; try eassumption;
-  eapply json_all_array_elements_smaller; 
-  simpl in *; eauto.
-Defined.
-
-Theorem Term_from_JSON_eq : forall `{Jsonifiable ASP, Jsonifiable Split} (js : JSON),
-  Term_from_JSON js = 
-    let type_name := "TERM" in
-    let type_str := type_name ++ "_" ++ type_string_constant in
-    let body_str := type_name ++ "_" ++ body_string_constant in
-    match (JSON_get_Object type_str js) with
-    | resultC (JSON_String cons_name) =>
-      if (eqb cons_name "asp") 
-      then 
-        asp_js <- (JSON_get_Object body_str js) ;;
-        asp_val <- from_JSON asp_js ;;
-        resultC (asp asp_val)
-      else if (eqb cons_name "att") 
-      then 
-        match (JSON_get_Object body_str js) as m' return (JSON_get_Object body_str js) = m' -> ResultT Term string with
-        | resultC (JSON_Array [JSON_String plc; term']) =>
-            fun _ =>
+      then match js with
+        | (JSON_Object [
+            _;
+            (_, JSON_Array [JSON_String plc; term'])
+          ]) =>
             plc_val <- from_string plc ;;
             term_val <- (Term_from_JSON term') ;;
             resultC (att plc_val term_val)
-        | resultC _ => fun _ => errC ("JSON Parsing 'att' ARGS: Incorrect number or wrong type of JSON args (expected [plc; term])")
-        | errC e => fun _ => errC e
-        end eq_refl
+        | _ => errC ("JSON Parsing 'att' ARGS: Incorrect number or wrong type of JSON args (expected [plc; term])")
+        end
       else if (eqb cons_name "lseq") 
-      then
-        match (JSON_get_Object body_str js) as m' return (JSON_get_Object body_str js) = m' -> ResultT Term string with
-        | resultC (JSON_Array [ term1; term2 ]) =>
-            fun _ =>
+      then match js with
+        | JSON_Object [
+            _;
+            (_, JSON_Array [ term1; term2 ])
+         ] =>
             term1_val <- (Term_from_JSON term1) ;;
             term2_val <- (Term_from_JSON term2) ;;
             resultC (lseq term1_val term2_val)
-        | resultC _ => fun _ => errC ("JSON Parsing 'lseq' ARGS: Incorrect number or wrong type of JSON args (expected [term1; term2])")
-        | errC e => fun _ => errC e
-        end eq_refl
+        | _ => errC ("JSON Parsing 'lseq' ARGS: Incorrect number or wrong type of JSON args (expected [term1; term2])")
+        end
       else if (eqb cons_name "bseq") 
-      then  
-        match (JSON_get_Object body_str js) as m' return (JSON_get_Object body_str js) = m' -> ResultT Term string with
-        | resultC (JSON_Array [ sp; term1; term2 ]) =>
-            fun _ =>
+      then match js with
+        | JSON_Object [
+            _;
+            (_, JSON_Array [ sp; term1; term2 ])
+          ] =>
             sp_val <- from_JSON sp ;;
             term1_val <- (Term_from_JSON term1) ;;
             term2_val <- (Term_from_JSON term2) ;;
             resultC (bseq sp_val term1_val term2_val)
-        | resultC _ => fun _ => errC ("JSON Parsing 'bseq' ARGS: Incorrect number or wrong type of JSON args (expected [sp; term1; term2])")
-        | errC e => fun _ => errC e
-        end eq_refl
+        | _ => errC ("JSON Parsing 'bseq' ARGS: Incorrect number or wrong type of JSON args (expected [sp; term1; term2])")
+        end
       else if (eqb cons_name "bpar") 
-      then  
-        match (JSON_get_Object body_str js) as m' return (JSON_get_Object body_str js) = m' -> ResultT Term string with
-        | resultC (JSON_Array [ sp; term1; term2 ]) =>
-            fun _ =>
+      then match js with
+        | JSON_Object [
+            _;
+            (_, JSON_Array [ sp; term1; term2 ])
+         ] =>
             sp_val <- from_JSON sp ;;
             term1_val <- (Term_from_JSON term1) ;;
             term2_val <- (Term_from_JSON term2) ;;
             resultC (bpar sp_val term1_val term2_val)
-        | resultC _ => fun _ => errC ("JSON Parsing 'bpar' ARGS: Incorrect number or wrong type of JSON args (expected [sp; term1; term2])")
-        | errC e => fun _ => errC e
-        end eq_refl
+        | _ => errC ("JSON Parsing 'bpar' ARGS: Incorrect number or wrong type of JSON args (expected [sp; term1; term2])")
+        end
       else errC "Invalid Term JSON constructor name"
     | resultC _ => errC "Invalid Term type"
     | errC e => errC e
     end.
-Proof.
-  intros; apply (Fix_eq json_depth_order_wf (fun _ => ResultT Term string)); intros; intuition;
-  repeat (break_match; eauto; intuition; eauto; try congruence;
-    try rewrite String.eqb_eq in *; subst; 
-    try rewrite String.eqb_neq in *; subst; try congruence
-  ).
-  - admit.
-  - admit. 
-  - admit.
-  - admit. 
-Admitted. 
 
 Global Instance Jsonifiable_Term `{Jsonifiable ASP, Jsonifiable Split} : Jsonifiable Term. 
 eapply Build_Jsonifiable with (to_JSON := Term_to_JSON) (from_JSON := Term_from_JSON).
-induction a; rewrite Term_from_JSON_eq; simpl in *;
+induction a; 
 repeat (result_monad_unfold;
 jsonifiable_hammer; repeat rewrite canonical_jsonification in *).
 Defined.
@@ -937,14 +619,7 @@ Fixpoint AppResultC_to_JSON `{Jsonifiable ASP_PARAMS, Jsonifiable Split, Jsonifi
       [(AppResultC_to_JSON res1); (AppResultC_to_JSON res2)]
   end.
 
-Definition AppResultC_from_JSON `{Jsonifiable ASP_PARAMS, Jsonifiable Split, Jsonifiable RawEv} (js : JSON) : ResultT AppResultC string.
-generalize js.
-refine (Fix json_depth_order_wf (fun _ => ResultT AppResultC string)
-  (
-    fun (js : JSON)
-      (rec : forall y : JSON,
-             lt (JSON_depth y) (JSON_depth js) ->
-             ResultT AppResultC string) =>
+Fixpoint AppResultC_from_JSON `{Jsonifiable ASP_PARAMS, Jsonifiable Split, Jsonifiable RawEv} (js : JSON) : ResultT AppResultC string :=
     let type_name := "AppResultC" in
     let type_str := type_name ++ "_" ++ type_string_constant in
     let body_str := type_name ++ "_" ++ body_string_constant in
@@ -953,160 +628,74 @@ refine (Fix json_depth_order_wf (fun _ => ResultT AppResultC string)
       if (eqb cons_name "mtc_app") 
       then resultC (mtc_app)
       else if (eqb cons_name "nnc_app") 
-      then 
-        match (JSON_get_Object body_str js) as m' return (JSON_get_Object body_str js) = m' -> ResultT AppResultC string with
-        | resultC (JSON_Array [JSON_String n; JSON_String bs]) =>
-            fun _ =>
+      then match js with
+        | JSON_Object [
+            _;
+            (_, JSON_Array [JSON_String n; JSON_String bs])
+         ] =>
             n_val <- from_string n ;;
             bs_val <- from_string bs ;;
             resultC (nnc_app n_val bs_val)
-        | resultC _ => fun _ => errC ("JSON Parsing 'nnc_app' ARGS: Incorrect number or wrong type of JSON args (expected [n; bs])")
-        | errC e => fun _ => errC e
-        end eq_refl
+        | _ => errC ("JSON Parsing 'nnc_app' ARGS: Incorrect number or wrong type of JSON args (expected [n; bs])")
+        end
       else if (eqb cons_name "ggc_app") 
-      then
-        match (JSON_get_Object body_str js) as m' return (JSON_get_Object body_str js) = m' -> ResultT AppResultC string with
-        | resultC (JSON_Array [ JSON_String plc; ps; rawev; res ]) =>
-            fun _ =>
-            plc_val <- from_string plc ;;
-            ps_val <- from_JSON ps ;;
-            rawev_val <- from_JSON rawev ;;
-            res_val <- (rec res _) ;;
-            resultC (ggc_app plc_val ps_val rawev_val res_val)
-        | resultC _ => fun _ => errC ("JSON Parsing 'ggc_app' ARGS: Incorrect number or wrong type of JSON args (expected [plc; ps; rawev; res])")
-        | errC e => fun _ => errC e
-        end eq_refl
-      else if (eqb cons_name "hhc_app") 
-      then
-        match (JSON_get_Object body_str js) as m' return (JSON_get_Object body_str js) = m' -> ResultT AppResultC string with
-        | resultC (JSON_Array [ JSON_String plc; ps; JSON_String bs; res ]) =>
-            fun _ =>
-            plc_val <- from_string plc ;;
-            ps_val <- from_JSON ps ;;
-            bs_val <- from_string bs ;;
-            res_val <- (rec res _) ;;
-            resultC (hhc_app plc_val ps_val bs_val res_val)
-        | resultC _ => fun _ => errC ("JSON Parsing 'hhc_app' ARGS: Incorrect number or wrong type of JSON args (expected [plc; ps; bs; res])")
-        | errC e => fun _ => errC e
-        end eq_refl
-      else if (eqb cons_name "eec_app") 
-      then
-        match (JSON_get_Object body_str js) as m' return (JSON_get_Object body_str js) = m' -> ResultT AppResultC string with
-        | resultC (JSON_Array [ JSON_String plc; ps; JSON_String bs; res ]) =>
-            fun _ =>
-            plc_val <- from_string plc ;;
-            ps_val <- from_JSON ps ;;
-            bs_val <- from_string bs ;;
-            res_val <- (rec res _) ;;
-            resultC (eec_app plc_val ps_val bs_val res_val)
-        | resultC _ => fun _ => errC ("JSON Parsing 'eec_app' ARGS: Incorrect number or wrong type of JSON args (expected [plc; ps; bs; res])")
-        | errC e => fun _ => errC e
-        end eq_refl
-      else if (eqb cons_name "ssc_app") 
-      then
-        match (JSON_get_Object body_str js) as m' return (JSON_get_Object body_str js) = m' -> ResultT AppResultC string with
-        | resultC (JSON_Array [ res1 ; res2 ]) =>
-            fun _ =>
-            res1_val <- (rec res1 _) ;;
-            res2_val <- (rec res2 _) ;;
-            resultC (ssc_app res1_val res2_val)
-        | resultC _ => fun _ => errC ("JSON Parsing 'ssc_app' ARGS: Incorrect number or wrong type of JSON args (expected [ res1 ; res2 ])")
-        | errC e => fun _ => errC e
-        end eq_refl
-      else errC "Invalid AppResultC JSON constructor name"
-    | resultC _ => errC "Invalid AppResultC type"
-    | errC e => errC e
-    end)); eapply json_get_object_result_always_smaller in e as E;
-  eapply PeanoNat.Nat.lt_trans; try eassumption;
-  eapply json_all_array_elements_smaller; 
-  simpl in *; eauto.
-Defined.
-
-Theorem AppResultC_from_JSON_eq : forall `{Jsonifiable ASP_PARAMS, Jsonifiable Split, Jsonifiable RawEv} (js : JSON),
-  AppResultC_from_JSON js = 
-    let type_name := "AppResultC" in
-    let type_str := type_name ++ "_" ++ type_string_constant in
-    let body_str := type_name ++ "_" ++ body_string_constant in
-    match (JSON_get_Object type_str js) with
-    | resultC (JSON_String cons_name) =>
-      if (eqb cons_name "mtc_app") 
-      then resultC (mtc_app)
-      else if (eqb cons_name "nnc_app") 
-      then 
-        match (JSON_get_Object body_str js) as m' return (JSON_get_Object body_str js) = m' -> ResultT AppResultC string with
-        | resultC (JSON_Array [JSON_String n; JSON_String bs]) =>
-            fun _ =>
-            n_val <- from_string n ;;
-            bs_val <- from_string bs ;;
-            resultC (nnc_app n_val bs_val)
-        | resultC _ => fun _ => errC ("JSON Parsing 'nnc_app' ARGS: Incorrect number or wrong type of JSON args (expected [n; bs])")
-        | errC e => fun _ => errC e
-        end eq_refl
-      else if (eqb cons_name "ggc_app") 
-      then
-        match (JSON_get_Object body_str js) as m' return (JSON_get_Object body_str js) = m' -> ResultT AppResultC string with
-        | resultC (JSON_Array [ JSON_String plc; ps; rawev; res ]) =>
-            fun _ =>
+      then match js with
+        | JSON_Object [
+            _;
+            (_, JSON_Array [ JSON_String plc; ps; rawev; res ]) 
+          ] =>
             plc_val <- from_string plc ;;
             ps_val <- from_JSON ps ;;
             rawev_val <- from_JSON rawev ;;
             res_val <- (AppResultC_from_JSON res) ;;
             resultC (ggc_app plc_val ps_val rawev_val res_val)
-        | resultC _ => fun _ => errC ("JSON Parsing 'ggc_app' ARGS: Incorrect number or wrong type of JSON args (expected [plc; ps; rawev; res])")
-        | errC e => fun _ => errC e
-        end eq_refl
+        | _ => errC ("JSON Parsing 'ggc_app' ARGS: Incorrect number or wrong type of JSON args (expected [plc; ps; rawev; res])")
+        end
       else if (eqb cons_name "hhc_app") 
-      then
-        match (JSON_get_Object body_str js) as m' return (JSON_get_Object body_str js) = m' -> ResultT AppResultC string with
-        | resultC (JSON_Array [ JSON_String plc; ps; JSON_String bs; res ]) =>
-            fun _ =>
+      then match js with
+        | JSON_Object [
+            _;
+            (_, JSON_Array [ JSON_String plc; ps; JSON_String bs; res ]) 
+          ] =>
             plc_val <- from_string plc ;;
             ps_val <- from_JSON ps ;;
             bs_val <- from_string bs ;;
             res_val <- (AppResultC_from_JSON res) ;;
             resultC (hhc_app plc_val ps_val bs_val res_val)
-        | resultC _ => fun _ => errC ("JSON Parsing 'hhc_app' ARGS: Incorrect number or wrong type of JSON args (expected [plc; ps; bs; res])")
-        | errC e => fun _ => errC e
-        end eq_refl
+          | _ => errC ("JSON Parsing 'hhc_app' ARGS: Incorrect number or wrong type of JSON args (expected [plc; ps; bs; res])")
+        end
       else if (eqb cons_name "eec_app") 
-      then
-        match (JSON_get_Object body_str js) as m' return (JSON_get_Object body_str js) = m' -> ResultT AppResultC string with
-        | resultC (JSON_Array [ JSON_String plc; ps; JSON_String bs; res ]) =>
-            fun _ =>
+      then match js with
+        | JSON_Object [
+            _;
+            (_, JSON_Array [ JSON_String plc; ps; JSON_String bs; res ]) 
+          ] =>
             plc_val <- from_string plc ;;
             ps_val <- from_JSON ps ;;
             bs_val <- from_string bs ;;
             res_val <- (AppResultC_from_JSON res) ;;
             resultC (eec_app plc_val ps_val bs_val res_val)
-        | resultC _ => fun _ => errC ("JSON Parsing 'eec_app' ARGS: Incorrect number or wrong type of JSON args (expected [plc; ps; bs; res])")
-        | errC e => fun _ => errC e
-        end eq_refl
+          | _ => errC ("JSON Parsing 'eec_app' ARGS: Incorrect number or wrong type of JSON args (expected [plc; ps; bs; res])")
+        end
       else if (eqb cons_name "ssc_app") 
-      then
-        match (JSON_get_Object body_str js) as m' return (JSON_get_Object body_str js) = m' -> ResultT AppResultC string with
-        | resultC (JSON_Array [ res1 ; res2 ]) =>
-            fun _ =>
+      then match js with
+        | JSON_Object [
+            _;
+            (_, JSON_Array [ res1; res2 ])
+          ] =>
             res1_val <- (AppResultC_from_JSON res1) ;;
             res2_val <- (AppResultC_from_JSON res2) ;;
             resultC (ssc_app res1_val res2_val)
-        | resultC _ => fun _ => errC ("JSON Parsing 'ssc_app' ARGS: Incorrect number or wrong type of JSON args (expected [ res1 ; res2 ])")
-        | errC e => fun _ => errC e
-        end eq_refl
+        | _ => errC ("JSON Parsing 'ssc_app' ARGS: Incorrect number or wrong type of JSON args (expected [ res1 ; res2 ])")
+        end
       else errC "Invalid AppResultC JSON constructor name"
     | resultC _ => errC "Invalid AppResultC type"
     | errC e => errC e
     end.
-Proof.
-  intros; apply (Fix_eq json_depth_order_wf (fun _ => ResultT AppResultC string)); intros; intuition;
-  repeat (break_match; eauto; intuition; eauto; try congruence;
-    try rewrite String.eqb_eq in *; subst; 
-    try rewrite String.eqb_neq in *; subst; try congruence
-  ); admit.
-Admitted. 
 
 Global Instance Jsonifiable_AppResultC `{Jsonifiable ASP_PARAMS, Jsonifiable Split, Jsonifiable RawEv} : Jsonifiable AppResultC.
 eapply Build_Jsonifiable with (to_JSON := AppResultC_to_JSON) (from_JSON := AppResultC_from_JSON).
-induction a; rewrite AppResultC_from_JSON_eq; simpl in *;
+induction a; simpl in *;
 repeat (result_monad_unfold;
 jsonifiable_hammer; repeat rewrite canonical_jsonification in *).
 Defined.
